sepcomp/CshmgenproofEFF.v
@@ -2506,7 +2506,7 @@ Lemma MATCH_afterExternal: forall
       (MatchMu: MATCH st1 mu st1 m1 st2 m2)
       (AtExtSrc : at_external (clight_eff_sem FE FE_FWD FE_UNCH) st1 = Some (e, ef_sig, vals1))
       (AtExtTgt : at_external csharpmin_eff_sem st2 = Some (e', ef_sig', vals2))
-      (ValInjMu : Forall2 (val_inject (as_inj mu)) vals1 vals2)
+      (ValInjMu : Forall2 (val_inject (restrict (as_inj mu) (vis mu))) vals1 vals2)
       (pubSrc' : block -> bool)
       (pubSrcHyp : pubSrc' =
                  (fun b : block => 
@@ -2658,12 +2658,12 @@ assert (RR1: REACH_closed m1'
            apply REACH_nil. unfold vis. rewrite Heql; trivial.
         specialize (RC _ Rb). unfold vis in RC.
            rewrite Heqq in RC; simpl in *.
-        assert (frgnBlocksSrc nu' b = true).
-          apply FRGnu'. rewrite replace_locals_frgnBlocksSrc. assumption.
+        rewrite replace_locals_frgnBlocksSrc in FRGnu'.
+        rewrite FRGnu' in RC.
         apply andb_true_iff.  
-        split. unfold DomSrc. rewrite (frgnBlocksSrc_extBlocksSrc _ WDnu' _ H). intuition.
+        split. unfold DomSrc. rewrite (frgnBlocksSrc_extBlocksSrc _ WDnu' _ RC). intuition.
         apply REACH_nil. unfold exportedSrc.
-          rewrite (frgnSrc_shared _ WDnu' _ H). intuition.
+          rewrite (frgnSrc_shared _ WDnu' _ RC). intuition.
   (*case DomSrc nu' b' &&
     (negb (locBlocksSrc nu' b') &&
      REACH m1' (exportedSrc nu' (ret1 :: nil)) b') = true*)
@@ -2705,14 +2705,15 @@ assert (GFnu': forall b, isGlobalBlock (Genv.globalenv prog) b = true ->
                DomSrc nu' b &&
                (negb (locBlocksSrc nu' b) && REACH m1' (exportedSrc nu' (ret1 :: nil)) b) = true).
      intros. specialize (Glob _ H).
-       assert (FF: frgnBlocksSrc nu' b = true).
-           eapply INC. rewrite replace_locals_frgnBlocksSrc. eassumption.
-       rewrite (frgnBlocksSrc_locBlocksSrc _ WDnu' _ FF). 
+       assert (FSRC:= extern_incr_frgnBlocksSrc _ _ INC).
+          rewrite replace_locals_frgnBlocksSrc in FSRC.
+       rewrite FSRC in Glob.
+       rewrite (frgnBlocksSrc_locBlocksSrc _ WDnu' _ Glob). 
        apply andb_true_iff; simpl.
         split.
-          unfold DomSrc. rewrite (frgnBlocksSrc_extBlocksSrc _ WDnu' _ FF). intuition.
+          unfold DomSrc. rewrite (frgnBlocksSrc_extBlocksSrc _ WDnu' _ Glob). intuition.
           apply REACH_nil. unfold exportedSrc.
-          rewrite (frgnSrc_shared _ WDnu' _ FF). intuition.
+          rewrite (frgnSrc_shared _ WDnu' _ Glob). intuition.
 split. 
   unfold vis in *.
   rewrite replace_externs_frgnBlocksSrc, replace_externs_locBlocksSrc in *.
@@ -2735,11 +2736,9 @@ split.
             destruct H9. right. rewrite H0 in H12.
               split; trivial.
               destruct (disjoint_extern_local _ WDnu' b); trivial. congruence.
-          (*rewrite replace_externs_frgnBlocksSrc, replace_externs_locBlocksSrc. *)
-          rewrite H3 in H11.
+          rewrite H3, H7 in H11.
             remember (locBlocksSrc nu' b) as d.
             destruct d; trivial; simpl in *.
-            apply H7 in H11.
             apply andb_true_iff.
             split. unfold DomSrc. rewrite (frgnBlocksSrc_extBlocksSrc _ WDnu' _ H11). intuition.
                apply REACH_nil. unfold exportedSrc. 
@@ -4308,15 +4307,13 @@ assert (GDE: genvs_domain_eq ge tge).
     destruct c1; inv H0. destruct k; inv H1.
     inv MC. exists res2.
     split. assumption.
-    split. eapply val_inject_incr; try eassumption.
-           apply restrict_incr.
+    split. eassumption.
     simpl. inv MK. trivial. }
 (* at_external*)
   { intros. destruct H as [MC [RC [PG [GFP [Glob [VAL [WD INJ]]]]]]].
     split; trivial.
     destruct c1; inv H0. destruct fd; inv H1.
     inv MC. simpl. exists args2; intuition. 
-      eapply forall_vals_inject_restrictD. 
       apply val_list_inject_forall_inject; eassumption.
     simpl.
     unfold transl_fundef in TR.
