sepcomp/effect_simulations_trans.v
@@ -167,15 +167,15 @@ Proof. (*follows structure of forward_simulations_trans.injinj*)
   destruct SIM12 
     as [core_data12 match_core12 core_ord12 core_ord_wf12 
       match_sm_wd12 genvs_dom_eq12 match_genv12
-      match_norm12 match_erase12 (*match_eraseUnknown12*)
-      match_validblock12 core_initial12 core_diagram12 eff_diagram12 
+      match_visible12 match_restrict12 
+      match_sm_valid12 (*match_protected12*) core_initial12 core_diagram12 eff_diagram12 
       strong_diagram12 strongperm_diagram12
       core_halted12 core_at_external12 eff_after_external12].  
   destruct SIM23 
     as [core_data23 match_core23 core_ord23 core_ord_wf23 
       match_sm_wd23 genvs_dom_eq23 match_genv23
-      match_norm23 match_erase23 (*match_eraseUnknown23*)
-      match_validblock23 core_initial23 core_diagram23 eff_diagram23
+      match_visible23 match_restrict23
+      match_sm_valid23 (*match_protected23*) core_initial23 core_diagram23 eff_diagram23
       strong_diagram23 strongperm_diagram23
       core_halted23 core_at_external23 eff_after_external23].
   eapply Build_SM_simulation_inject with
@@ -230,75 +230,22 @@ Proof. (*follows structure of forward_simulations_trans.injinj*)
          rewrite compose_sm_extern.
          solve [eapply meminj_preserves_globals_ind_compose; eassumption].
   apply GE12b.
- (*match_norm*)
-    clear - match_norm12 match_norm23 match_sm_wd12 match_sm_wd23.
+ (*match_visible*)
+    clear - match_sm_wd12 match_visible12.
     intros. rename c2 into c3. rename m2 into m3.
       destruct d as [[d12 cc2] d23].
       destruct H as [c2 [m2 [mu12 [mu23 [X [J [INV [MC12 MC23]]]]]]]]; subst.
-      simpl. rewrite vis_compose_sm. eapply match_norm12. eassumption. (*
-    specialize (match_norm23 _ _ _ _ _ _ MC23 downstreamMu H0).
-    specialize (match_norm12 _ _ _ _ _ _ MC12 (sm_extern_normalize mu23 downstreamMu)).
-    exists c2, m2.
-    exists (sm_extern_normalize mu12 (sm_extern_normalize mu23 downstreamMu)). 
-    exists (sm_extern_normalize mu23 downstreamMu). 
-    simpl in *. split. trivial. 
-    rewrite sm_extern_normalize_locBlocksTgt, sm_extern_normalize_extBlocksTgt,
-                    sm_extern_normalize_pubBlocksTgt, sm_extern_normalize_frgnBlocksTgt. 
-    rewrite sm_extern_normalize_locBlocksSrc, sm_extern_normalize_extBlocksSrc,
-                    sm_extern_normalize_pubBlocksSrc, sm_extern_normalize_frgnBlocksSrc.
-    split. destruct mu12; simpl in *. unfold compose_sm; simpl.
-            rewrite sm_extern_normalize_locBlocksTgt, sm_extern_normalize_extBlocksTgt,
-                    sm_extern_normalize_pubBlocksTgt, sm_extern_normalize_frgnBlocksTgt.
-           destruct mu23; simpl in *. rewrite <- normalize_compose_commute. 
-           eapply f_equal.
-       trivial.
-    split. apply INV.
-    split; try assumption.
-    apply match_norm12.
-      split. eapply sm_extern_normalize_WD.
-                eauto. apply H0. apply H0.
-      rewrite sm_extern_normalize_locBlocksSrc, sm_extern_normalize_extBlocksSrc,
-              sm_extern_normalize_pubBlocksSrc, sm_extern_normalize_frgnBlocksSrc.
-      apply INV. *)
- (*TrimUnknown
-    clear match_norm12 match_norm23 core_diagram23  core_halted23 
-       core_at_external23 (*eff_after_external23 *)
-    core_diagram12  core_halted12 core_at_external12 (*eff_after_external12*)
-    eff_diagram12 eff_diagram23 strong_diagram12 strong_diagram23.
-    clear eff_after_external23 (*eff_after_external_ModEffects12 *)
-     core_initial23  (*eff_after_external_ModEffects23 *)
-     eff_after_external12 core_initial12.
-    intros. rename c2 into c3.  rename m2 into m3.
-    destruct d as [[d12 cc2] d23].
-    destruct H as [c2 [m2 [mu12 [mu23 [X [J [INV [MC12 MC23]]]]]]]]; subst.??*)
- (*eraseUnknown
-    clear match_norm12 match_norm23 core_diagram23  core_halted23 
-       core_at_external23 (*eff_after_external23 *)
-    core_diagram12  core_halted12 core_at_external12 (*eff_after_external12*)
-    eff_diagram12 eff_diagram23 strong_diagram12 strong_diagram23.
-    clear eff_after_external23 (*eff_after_external_ModEffects12 *)
-     core_initial23  (*eff_after_external_ModEffects23 *)
-     eff_after_external12 core_initial12.
-    intros. rename c2 into c3.  rename m2 into m3.
-    destruct d as [[d12 cc2] d23].
-    destruct H as [c2 [m2 [mu12 [mu23 [X [J [INV [MC12 MC23]]]]]]]]; subst.
-    specialize (match_eraseUnknown12 _ _ _ _ _ _ MC12).
-    specialize (match_eraseUnknown23 _ _ _ _ _ _ MC23).
-    exists c2, m2, (EraseUnknown mu12), (EraseUnknown mu23).
-    split; trivial.
-    split. eapply compose_sm_EraseUnknown. eauto. eapply INV.
-    split. destruct mu12; destruct mu23; simpl in *. apply INV.
-    split; assumption.*)
+      simpl. rewrite vis_compose_sm. eapply match_visible12. eassumption. 
  (*match_restrict*)
-    clear - match_erase12 match_erase23.
+    clear - match_restrict12.
     intros. rename c2 into c3. rename m2 into m3.
     destruct d as [[d12 cc2] d23].
     destruct H as [c2 [m2 [mu12 [mu23 [XX [J [INV [MC12 MC23]]]]]]]]; subst.
     simpl in *.
     exists c2, m2, (restrict_sm mu12 X), mu23.
-    specialize (match_erase12 _ _ _ _ _ _ X MC12 H0 H1).
+    specialize (match_restrict12 _ _ _ _ _ _ X MC12 H0 H1).
     intuition.
-    unfold compose_sm; simpl. 
+    unfold compose_sm; simpl.
     f_equal; try (destruct mu12; reflexivity).
       destruct mu12; simpl in *.
         unfold compose_meminj, restrict. extensionality b.
@@ -312,82 +259,25 @@ Proof. (*follows structure of forward_simulations_trans.injinj*)
       destruct mu12; simpl in *. assumption.
       destruct mu12; simpl in *. apply (H2 _ H4).
       destruct mu12; simpl in *. apply (H5 _ H4).
- (*match_erase
-    clear - match_erase12 match_erase23.
-    intros. rename c2 into c3. rename m2 into m3.
-    destruct d as [[d12 cc2] d23].
-    destruct H as [c2 [m2 [mu12 [mu23 [XX [J [INV [MC12 MC23]]]]]]]]; subst.
-     (*assert (ER12: erasable mu12 m1 (fun b => X b && negb(mapped (as_inj mu12) b))).
-      destruct H0 as [ERa ERb]; simpl in ERa, ERb.
-      split; intros.
-         intros b Hb. remember (mapped (as_inj mu12) b).
-              destruct b0; simpl. rewrite negb_true_iff. rewrite andb_false_r. trivial.
-         apply REACHAX in Hb. destruct Hb as [L HL].
-         generalize dependent b.
-         induction L; simpl; intros; inv HL.
-             rewrite andb_true_iff in H.
-             rewrite negb_true_iff in H. destruct H.
-             congruence.
-         specialize (IHL _ H1); clear H1.
-           remember (mapped (as_inj mu12) b') as d.
-           destruct d. 
-      split; assumption.
-    specialize (match_erase12 _ _ _ _ _ _ _ MC12 ER12).
-    exists c2, m2, (Erase mu12 X). exists mu23.
-    simpl. intuition.
-      unfold Erase, compose_sm; simpl. destruct mu12; simpl in *.
-        f_equal. extensionality b. 
-        unfold compose_meminj.
-        remember (X b) as d.
-        destruct d; trivial. 
-      unfold Erase; simpl. destruct mu12; simpl in *. assumption.
-      unfold Erase; simpl. destruct mu12; simpl in *. assumption.
-      unfold Erase in H3; simpl. destruct mu12; simpl in *. apply (H1 _ H3).
-      unfold Erase in H3; simpl. destruct mu12; simpl in *. apply (H4 _ H3).*)
- *)(*match_erase
-    clear - match_erase12 match_erase23.
-    intros. rename c2 into c3. rename m2 into m3.
-    destruct d as [[d12 cc2] d23].
-    destruct H as [c2 [m2 [mu12 [mu23 [XX [J [INV [MC12 MC23]]]]]]]]; subst.
-    assert (ER12: erasable mu12 m1 X).
-      destruct H0 as [ERa ERb]; simpl in ERa, ERb.
-      split; assumption.
-    specialize (match_erase12 _ _ _ _ _ _ _ MC12 ER12).
-    exists c2, m2, (Erase mu12 X). exists mu23.
-    simpl. intuition.
-      unfold Erase, compose_sm; simpl. destruct mu12; simpl in *.
-        f_equal. extensionality b. 
-        unfold compose_meminj.
-        remember (X b) as d.
-        destruct d; trivial. 
-      unfold Erase; simpl. destruct mu12; simpl in *. assumption.
-      unfold Erase; simpl. destruct mu12; simpl in *. assumption.
-      unfold Erase in H3; simpl. destruct mu12; simpl in *. apply (H1 _ H3).
-      unfold Erase in H3; simpl. destruct mu12; simpl in *. apply (H4 _ H3).*)
  (*sm_valid*)
-    clear genvs_dom_eq12 match_genv12 genvs_dom_eq23 match_genv23 
-       match_norm12 match_norm23 core_diagram23  core_halted23 
-       core_at_external23 (*eff_after_external23 *)
-       core_diagram12  core_halted12 core_at_external12 (*eff_after_external12*)
-       eff_diagram12 eff_diagram23 strong_diagram12 strong_diagram23.
-    clear eff_after_external23 (*eff_after_external_ModEffects12 *)
-     core_initial23  (*eff_after_external_ModEffects23 *)
-     eff_after_external12 core_initial12.
+    clear - match_sm_valid12 match_sm_valid23.
     intros. rename c2 into c3.  rename m2 into m3.
     destruct d as [[d12 cc2] d23].
     destruct H as [c2 [m2 [mu12 [mu23 [X [J [INV [MC12 MC23]]]]]]]]; subst.
-    specialize (match_validblock12 _ _ _ _ _ _ MC12).
-    specialize (match_validblock23 _ _ _ _ _ _ MC23).
+    specialize (match_sm_valid12 _ _ _ _ _ _ MC12).
+    specialize (match_sm_valid23 _ _ _ _ _ _ MC23).
     unfold sm_valid, compose_sm. destruct mu12; destruct mu23; simpl in *.
-    split; intros. eapply match_validblock12. apply H.
-    eapply match_validblock23. apply H.
+    split; intros. eapply match_sm_valid12. apply H.
+    eapply match_sm_valid23. apply H.
+ (*match_protected
+    clear - match_sm_wd12 match_protected12
+            match_sm_wd23 match_protected23.
+    intros. rename c2 into c3.  rename m2 into m3.
+    destruct d as [[d12 cc2] d23].
+    destruct H as [c2 [m2 [mu12 [mu23 [X [J [INV [MC12 MC23]]]]]]]]; subst.
+    simpl. apply (match_protected12 _ _ _ _ _ _ MC12 _ H0 H1).*)
  (*initial_core*)
-   clear match_genv12  match_genv23 
-     core_diagram23  core_halted23 core_at_external23 
-     eff_after_external23 
-     core_diagram12  core_halted12 core_at_external12 eff_after_external12
-     eff_diagram12 eff_diagram23 strong_diagram12 strong_diagram23
-     strongperm_diagram12 strongperm_diagram23.
+   clear - EPC genvs_dom_eq12 core_initial12 genvs_dom_eq23 core_initial23.
    intros. rename m2 into m3. rename v2 into v3. rename vals2 into vals3. 
     rewrite (EPC v1 v3 sig) in H. destruct H as [v2 [EP12 EP23]].
     (*assert (HT: Forall2 Val.has_type vals1 (sig_args sig)). 
@@ -512,54 +402,35 @@ Proof. (*follows structure of forward_simulations_trans.injinj*)
   split. subst; simpl. repeat (split; trivial).
   split; trivial. 
  (*core_diagram*)
-  clear match_norm12 match_norm23 core_initial23 core_halted23 core_at_external23 
-    (*eff_after_external23*)
-    core_initial12  core_halted12 core_at_external12 (*eff_after_external12*)
-    EPC epts12 epts23 epts13 eff_diagram12 eff_diagram23
-   eff_after_external12 eff_after_external23 strong_diagram12 strong_diagram23
-   (*eff_after_external_ModEffects12 eff_after_external_ModEffects23*).
+  clear - match_sm_wd12 match_sm_valid12 core_diagram12 
+          match_sm_wd23 match_sm_valid23 core_diagram23.
   intros. rename st2 into st3. rename m2 into m3.
   destruct cd as [[d12 cc2] d23].
   destruct H0 as [c2 [m2 [mu12 [mu23 [X [J [INV [MC12 MC23]]]]]]]]; subst.
   eapply diagram_injinj; try eassumption.
  (*eff_diagram*)
-  clear core_initial23 match_norm12 match_norm23 core_halted23 core_at_external23 
-   (*eff_after_external23*)
-    core_initial12  core_halted12 core_at_external12 (*eff_after_external12*)
-    EPC epts12 epts23 epts13 core_diagram12 core_diagram23
-    eff_after_external12 eff_after_external23 strong_diagram12 strong_diagram23
-    (*eff_after_external_ModEffects12 eff_after_external_ModEffects23*).
+  clear - match_sm_wd12 match_sm_valid12 eff_diagram12 
+          match_sm_wd23 match_sm_valid23 eff_diagram23.
   intros. rename st2 into st3. rename m2 into m3.
   destruct cd as [[d12 cc2] d23].
-  destruct H0 as [c2 [m2 [j12 [j23 [X [J [INV [MC12 MC23]]]]]]]]; subst.
+  destruct H0 as [c2 [m2 [mu12 [mu23 [X [J [INV [MC12 MC23]]]]]]]]; subst.
   eapply effdiagram_injinj; try eassumption.
  (*strong_diagram*)
-  clear core_initial23 match_norm12 match_norm23 core_halted23 core_at_external23 
-    (*eff_after_external23*)
-    core_initial12  core_halted12 core_at_external12 (*eff_after_external12*)
-    EPC epts12 epts23 epts13 core_diagram12 core_diagram23
-    eff_after_external12 eff_after_external23 eff_diagram12 eff_diagram23
-    (*eff_after_external_ModEffects12 eff_after_external_ModEffects23*).
+  clear - match_sm_wd12 match_sm_valid12 strong_diagram12 
+          match_sm_wd23 match_sm_valid23 strong_diagram23.
   intros. rename st2 into st3. rename m2 into m3.
   destruct cd as [[d12 cc2] d23].
-  destruct H0 as [c2 [m2 [j12 [j23 [X [J [INV [MC12 MC23]]]]]]]]; subst.
-  eapply effdiagram_strong_injinj; try eassumption.
+  destruct H0 as [c2 [m2 [mu12 [mu23 [X [J [INV [MC12 MC23]]]]]]]]; subst.
+  eapply effdiagram_strong_injinj; try eassumption. 
  (*strongperm_diagram*)
-  clear core_initial23 match_norm12 match_norm23 core_halted23 core_at_external23 
-    (*eff_after_external23*) strong_diagram12 strong_diagram23
-    core_initial12  core_halted12 core_at_external12 (*eff_after_external12*)
-    EPC epts12 epts23 epts13 core_diagram12 core_diagram23
-    eff_after_external12 eff_after_external23 eff_diagram12 eff_diagram23
-    (*eff_after_external_ModEffects12 eff_after_external_ModEffects23*).
+  clear - match_sm_wd12 match_sm_valid12 strongperm_diagram12 
+          match_sm_wd23 match_sm_valid23 strongperm_diagram23.
   intros. rename st2 into st3. rename m2 into m3.
   destruct cd as [[d12 cc2] d23].
-  destruct H0 as [c2 [m2 [j12 [j23 [X [J [INV [MC12 MC23]]]]]]]]; subst.
+  destruct H0 as [c2 [m2 [mu12 [mu23 [X [J [INV [MC12 MC23]]]]]]]]; subst.
   eapply effdiagram_strong_perm_injinj; eassumption.
 (*halted*)
-  clear match_norm12 match_norm23 core_initial23 core_at_external23 eff_after_external23
-    core_initial12  core_at_external12 eff_after_external12
-    EPC epts12 epts23 epts13 core_diagram12 core_diagram23
-    eff_diagram12 eff_diagram23 strong_diagram12 strong_diagram23.
+  clear - match_sm_wd12 core_halted12 match_sm_wd23 core_halted23.
   intros. rename c2 into c3. rename m2 into m3.  
   destruct cd as [[d12 cc2] d23].
   destruct H as [c2 [m2 [mu12 [mu23 [X [J [INV [MC12 MC23]]]]]]]]; subst.
@@ -575,14 +446,13 @@ Proof. (*follows structure of forward_simulations_trans.injinj*)
   split. rewrite compose_sm_as_inj; trivial.
            eapply Mem.inject_compose; eassumption.   
   split. rewrite compose_sm_as_inj; trivial.
-           eapply val_inject_compose; eassumption.
+         rewrite restrict_compose, vis_compose_sm; simpl.
+         eapply val_inject_compose; try eassumption.
+         eapply val_inject_incr; try eassumption.
+         apply restrict_incr.
   assumption.
-
 (*at_external*)
-  clear match_norm12 match_norm23 core_initial23 core_halted23 eff_after_external23 
-    core_initial12  core_halted12 eff_after_external12
-    EPC epts12 epts23 epts13 core_diagram12 core_diagram23
-    eff_diagram12 eff_diagram23.
+  clear - match_sm_wd12 core_at_external12 match_sm_wd23 core_at_external23.
   intros. rename c2 into c3. rename m2 into m3.
   rename H0 into AtExtSrc. 
   destruct cd as [[d12 cc2] d23]. 
@@ -595,266 +465,16 @@ Proof. (*follows structure of forward_simulations_trans.injinj*)
   rewrite compose_sm_as_inj; try eauto.   
     split. eapply Mem.inject_compose; eassumption.
     exists vals3.
-    split. eapply forall_val_inject_compose; eassumption.
+    split. rewrite restrict_compose, vis_compose_sm; simpl.
+           eapply forall_val_inject_compose; try eassumption.
+           eapply forall_vals_inject_restrictD; eassumption.
     (*split;*) assumption.
   eapply GLUEINV. 
-  eapply GLUEINV. 
-(*eff_after_external - version using match_eraseUnknown
-  clear core_diagram12 core_initial12 core_halted12 eff_diagram12 
-        core_diagram23 core_initial23 core_halted23 eff_diagram23
-        (*eff_after_external12 eff_after_external23
-        eff_after_external_ModEffects12 eff_after_external_ModEffects23*)
-        strong_diagram23 strong_diagram12 match_norm12 match_norm23.
-    (*core_at_externalFAT1*) (*FAT0 core_at_externalFAT0*) 
-  intros. rename st2 into st3. rename m2 into m3. 
-          rename vals2 into vals3'. rename m2' into m3'.
-          rename UnchLOOR into UnchLOOR13.
-  destruct cd as [[d12 cc2] d23].
-  destruct MatchMu as [st2 [m2 [mu12 [mu23 [Hst2 [HMu [GLUEINV [MC12 MC23]]]]]]]].
-  specialize (match_eraseUnknown12 _ _ _ _ _ _ MC12). 
-  specialize (match_eraseUnknown23 _ _ _ _ _ _ MC23). clear match_eraseUnknown23.
-  assert (WDmu12:= match_sm_wd12 _ _ _ _ _ _ MC12).
-  clear MC12. remember (EraseUnknown mu12) as nmu12.
-  assert (WDnmu12:= match_sm_wd12 _ _ _ _ _ _ match_eraseUnknown12).
-  assert (WDmu23:= match_sm_wd23 _ _ _ _ _ _ MC23).
-  assert (HmuNorm: mu = compose_sm nmu12 mu23).
-     subst. apply sm_extern_normalize_compose_sm.
-  clear HMu.
-  assert (WDmu: SM_wd (compose_sm nmu12 mu23)).
-    eapply compose_sm_wd; try eassumption.
-      subst. rewrite sm_extern_normalize_pubBlocksTgt. apply GLUEINV.
-      subst. rewrite sm_extern_normalize_frgnBlocksTgt. apply GLUEINV.
-  clear match_norm12.
-  assert (mu12_valid:= match_validblock12 _ _ _ _ _ _ NormMC12).
-  assert (mu23_valid:= match_validblock23 _ _ _ _ _ _ MC23).
-  rename ret2 into ret3.  
-  destruct (core_at_external12 _ _ _ _ _ _ _ _ _ NormMC12 AtExtSrc)
-   as [MInj12 [vals2 [ArgsInj12 [ArgsHT2 AtExt2]]]]; clear core_at_external12.
-  destruct (core_at_external23 _ _ _ _ _ _ _ _ _ MC23 AtExt2)
-   as [MInj23 [vals3 [ArgsInj23 [ArgsHT3 AtExt3]]]]; clear core_at_external23.
-  
-  (*Prove uniqueness of e, ef_sig, vals3. We do this by hand, instead of 
-     rewrite AtExtTgt in AtExt3; inv Atext3 in order to avoid the subst
-     taht's inherent in inv AtExt3. Probably there's a better way to do this..*)
-  assert (e' = e /\ ef_sig' = ef_sig /\ vals3'=vals3).
-     rewrite AtExtTgt in AtExt3. inv AtExt3. intuition.
-  destruct H as [HH1 [HH2 HH3]].
-  rewrite HH1, HH2, HH3 in *. clear HH1 HH2 HH3 e' ef_sig' vals3' AtExt3.
-
-  (*clear MemInjMu. follows from MInj12 MInj23*)
-  specialize (eff_after_external12 _ _ _ _ _ _ _ _ _ _ _ _ MInj12 
-        NormMC12 AtExtSrc AtExt2 ArgsInj12
-        _ (eq_refl _) _ (eq_refl _) _ (eq_refl _)). 
-  specialize (eff_after_external23 _ _ _ _ _ _ _ _ _ 
-      _ _ _ MInj23 MC23 AtExt2 AtExtTgt ArgsInj23 _ (eq_refl _) 
-      _ (eq_refl _) _ (eq_refl _)).
-  assert (LeakedCompSrc: locBlocksSrc mu = locBlocksSrc nmu12 /\
-                        exportedSrc mu vals1 = exportedSrc nmu12 vals1). 
-     subst. clear - WDnmu12 WDmu. simpl.  
-        rewrite sm_extern_normalize_locBlocksSrc.
-        unfold exportedSrc. 
-        rewrite sharedSrc_iff_frgnpub; trivial. simpl. 
-        rewrite sharedSrc_iff_frgnpub; trivial.
-        rewrite sm_extern_normalize_frgnBlocksSrc, sm_extern_normalize_pubBlocksSrc.
-        intuition.
-  destruct LeakedCompSrc as [LSa LSb]. rewrite LSa, LSb in *. clear LSa LSb.
-  assert (LeakedCompTgt: locBlocksTgt mu = locBlocksTgt mu23 
-                       /\ exportedTgt mu vals3 = exportedTgt mu23 vals3).
-     subst. clear - WDmu23 WDmu. simpl.  
-        unfold exportedTgt, sharedTgt. simpl. intuition. 
-  destruct LeakedCompTgt as [LTa LTb]. rewrite LTa, LTb in *. clear LTa LTb.
-   remember (fun b => locBlocksTgt nmu12 b && 
-             REACH m2 (exportedTgt nmu12 vals2) b) as pubTgtMid'.
-   remember (fun b => locBlocksSrc mu23 b && 
-             REACH m2 (exportedSrc mu23 vals2) b) as pubSrcMid'.
-   assert (MID: forall b, pubTgtMid' b = true -> pubSrcMid' b = true).
-        clear eff_after_external12 match_validblock23 eff_after_external23.
-        rewrite HeqpubTgtMid', HeqpubSrcMid'. 
-        destruct GLUEINV as [? [? [? ?]]].
-        subst.
-        rewrite sm_extern_normalize_locBlocksTgt, sm_extern_normalize_exportedTgt; trivial.
-           rewrite H0. intros. rewrite andb_true_iff in *.
-        destruct H3. split; trivial.
-        eapply REACH_mono; try eassumption.
-        unfold exportedTgt, exportedSrc, sharedTgt.
-        rewrite sharedSrc_iff_frgnpub; trivial.
-        intros. repeat rewrite orb_true_iff in *.
-        intuition.
-  assert (NU: nu = compose_sm (replace_locals nmu12 pubSrc' pubTgtMid')
-              (replace_locals mu23 pubSrcMid' pubTgt')).
-     clear frgnSrcHyp frgnTgtHyp eff_after_external23.
-     subst. unfold compose_sm; simpl.
-     rewrite replace_locals_extern, replace_locals_local,
-             replace_locals_locBlocksSrc, replace_locals_locBlocksTgt,
-            replace_locals_pubBlocksSrc, replace_locals_pubBlocksTgt,
-            replace_locals_frgnBlocksSrc, replace_locals_frgnBlocksTgt,
-            replace_locals_DomSrc, replace_locals_DomTgt.
-     rewrite replace_locals_extern, replace_locals_local.
-     rewrite sm_extern_normalize_DomSrc, sm_extern_normalize_locBlocksSrc,
-             sm_extern_normalize_local, sm_extern_normalize_extern.
-     f_equal. 
-
-  clear NuHyp.
-  (*produce all the hypothesis necessary for applying interpolation*)
-  assert (MinjNu12: Mem.inject (as_inj (replace_locals nmu12 pubSrc' pubTgtMid')) m1 m2).
-     rewrite replace_locals_as_inj. assumption.
-  assert (MinjNu23: Mem.inject (as_inj (replace_locals mu23 pubSrcMid' pubTgt')) m2 m3).
-     rewrite replace_locals_as_inj. assumption.
-  assert (WDnu12: SM_wd (replace_locals nmu12 pubSrc' pubTgtMid')).
-       subst.
-       eapply replace_locals_wd; try eassumption.
-         intros. apply andb_true_iff in H.
-           destruct H as [locB R].
-           destruct (REACH_local_REACH _ WDnmu12 _ _ _ _ 
-              MInj12 ArgsInj12 _ R locB) as [b2 [d1 [LOC12 R2]]].
-           exists b2, d1; split; trivial.
-           rewrite andb_true_iff, R2.
-           split; trivial.
-           eapply local_locBlocks; eassumption.
-         intros. apply andb_true_iff in H. apply H. 
-  assert (WDnu23: SM_wd (replace_locals mu23 pubSrcMid' pubTgt')).
-       subst. 
-       eapply replace_locals_wd; try eassumption.
-       destruct GLUEINV as [GIa [GIb [GIc GId]]]. subst. 
-       intros b2; intros. apply andb_true_iff in H.
-           destruct H as [locB R].
-           destruct (REACH_local_REACH _ WDmu23 _ _ _ _ 
-              MInj23 ArgsInj23 _ R locB) as [b3 [d2 [LOC23 R3]]].
-           exists b3, d2; split; trivial.
-           rewrite andb_true_iff, R3.
-           split; trivial.
-           eapply local_locBlocks; eassumption.
-         intros. apply andb_true_iff in H. apply H.
-  assert (nu12_valid: sm_valid (replace_locals nmu12 pubSrc' pubTgtMid') m1 m2).
-     split. rewrite replace_locals_DOM. eapply mu12_valid.
-     rewrite replace_locals_RNG. eapply mu12_valid.
-  assert (nu23_valid: sm_valid (replace_locals mu23 pubSrcMid' pubTgt') m2 m3).
-     split. rewrite replace_locals_DOM. eapply mu23_valid.
-     rewrite replace_locals_RNG. eapply mu23_valid.
-  rewrite NU in INC, SEP.
-  destruct (EFFAX.effect_interp_II _ _ _ MinjNu12 _ FwdSrc
-      _ _ MinjNu23 _ FwdTgt nu' WDnu' SMvalNu' MemInjNu'
-      INC SEP nu12_valid nu23_valid)
-     as [m2' [nu12' [nu23' [X [Incr12 [Incr23 [MInj12'
-        [Fwd2 [MInj23' [Sep12 [Sep23 [nu12'valid
-        [nu23'valid [GLUEINV' [Norm' [UnchMidA
-        [UnchMidB UnchMidC]]]]]]]]]]]]]]]]]; simpl in *.
-    (*discharge the unchOn application conditions*)
-       subst; apply UnchPrivSrc.
-       subst. apply UnchLOOR13. 
-    (*discharge the GLUE application condition*)
-      rewrite replace_locals_DomSrc, replace_locals_DomTgt,
-            replace_locals_locBlocksSrc, replace_locals_locBlocksTgt,
-            replace_locals_pubBlocksSrc, replace_locals_pubBlocksTgt,
-            replace_locals_frgnBlocksSrc, replace_locals_frgnBlocksTgt.
-      destruct GLUEINV as [GLUEa [GLUEb [GLUEc GLUEd]]].
-      repeat (split; trivial).
-      subst. rewrite sm_extern_normalize_DomTgt; trivial.
-      subst. rewrite sm_extern_normalize_locBlocksTgt; trivial.
-      subst. rewrite sm_extern_normalize_frgnBlocksTgt; trivial.
-    (*discharge the Norm Hypothesis*)
-      rewrite Heqnmu12. do 2 rewrite replace_locals_extern.
-      intros.
-      destruct (sm_extern_normalize_norm _ _ _ _ _ H) as [EXT1 [[b3 d2] EXT2]].
-      exists b3, d2; trivial.
-
-  (*next, prepare for application of eff_after_external12*)
-  destruct GLUEINV' as [WDnu12' [WDnu23' [GLUEa' [GLUEb' [GLUEc' GLUEd']]]]].
-  assert (exists ret2, val_inject (as_inj nu12') ret1 ret2 /\ 
-                       val_inject (as_inj nu23') ret2 ret3 /\
-                       Val.has_type ret2 (proj_sig_res ef_sig)(* /\
-                       val_valid ret2 m2'*)). 
-    subst. rewrite compose_sm_as_inj in RValInjNu'; trivial.
-    destruct (val_inject_split _ _ _ _ RValInjNu')
-      as [ret2 [RValInjNu12' RValInjNu23']].  
-    exists ret2. repeat (split; trivial).
-    eapply valinject_hastype; eassumption.
-  destruct H as [ret2 [RValInjNu12' [RValInjNu23' RetType2]]].
-  subst. 
-  specialize (eff_after_external12 nu12' ret1 
-     m1' ret2 m2' Incr12 Sep12 WDnu12' nu12'valid MInj12' RValInjNu12'
-     FwdSrc Fwd2 RetType2).
-
-  destruct (eff_after_external12 _ (eq_refl _) 
-      _ (eq_refl _) _ (eq_refl _))
-    as [d12' [c1' [c2' [AftExt1 [AftExt2 MC12']]]]]; clear eff_after_external12.
-   (*discharge unchangedOn-application conditions*)
-      apply UnchPrivSrc.
-      apply UnchMidB.
-
-  (*next, apply eff_after_external23*)
-  specialize (eff_after_external23 nu23').
-  destruct (eff_after_external23 ret2 m2' 
-       ret3 m3' Incr23 Sep23 WDnu23' nu23'valid
-       MInj23' RValInjNu23' Fwd2 FwdTgt RetTypeTgt
-     _ (eq_refl _) _ (eq_refl _) _ (eq_refl _)) as
-     [d23' [c22' [c3' [AftExt22 [AftExt3 MC23']]]]];
-    subst; clear eff_after_external23.
-    (*discharge unchangedOn application conditions*)
-      apply UnchMidA.
-      apply UnchMidC.
-
-  (*finally, instantiate the existentials, and establish conclusion*)
-  rewrite AftExt22 in AftExt2. inv AftExt2.
-  clear GLUEINV.
-  exists (d12', Some c2', d23').
-  exists c1'. exists c3'.
-  split. assumption.
-  split. assumption.
-  exists c2'. exists m2'.
-  exists (replace_externs nu12'
-            (fun b => DomSrc nu12' b && (negb (locBlocksSrc nu12' b) 
-                                     && REACH m1' (exportedSrc nu12' (ret1::nil)) b))
-            (fun b => DomTgt nu12' b && (negb (locBlocksTgt nu12' b) 
-                                     && REACH m2' (exportedTgt nu12' (ret2::nil)) b))).
-  exists (replace_externs nu23'
-            (fun b => DomSrc nu23' b && (negb (locBlocksSrc nu23' b) 
-                                     && REACH m2' (exportedSrc nu23' (ret2::nil)) b))
-            (fun b => DomTgt nu23' b && (negb (locBlocksTgt nu23' b) 
-                                     && REACH m3' (exportedTgt nu23' (ret3::nil)) b))).
-  split. reflexivity.
-  unfold compose_sm. simpl.
-         repeat rewrite replace_externs_DomSrc, replace_externs_DomTgt, 
-                 replace_externs_locBlocksSrc, replace_externs_locBlocksTgt,
-                 replace_externs_pubBlocksSrc, replace_externs_pubBlocksTgt,  
-                 replace_externs_frgnBlocksSrc, replace_externs_frgnBlocksTgt.
-        rewrite replace_externs_extern, replace_externs_local.
-        rewrite replace_externs_extern, replace_externs_local.
-  split. f_equal; trivial. 
-         unfold exportedSrc; simpl.
-           rewrite sharedSrc_iff_frgnpub; trivial.
-           rewrite sharedSrc_iff_frgnpub; trivial.
-  clear UnchLOOR13 UnchPrivSrc SEP INC MID UnchMidB Incr12 
-        Sep12 WDnu12 nu12_valid MinjNu12 UnchMidC UnchMidA Sep23
-        Incr23 nu23_valid WDnu23 MinjNu23 MemInjMu ValInjMu.
-  split. 
-    clear MC23' MC12'.
-    repeat (split; trivial).
-    rewrite GLUEa', GLUEb'.
-         intros. do 2 rewrite andb_true_iff.
-                 do 2 rewrite andb_true_iff in H.
-                 destruct H as [HH1 [HH2 HH3]].
-                 split; trivial. split; trivial.
-                 eapply REACH_mono; try eassumption.
-                 unfold exportedTgt, exportedSrc; intros.
-                 apply orb_true_iff. apply orb_true_iff in H.
-                 destruct H.
-                   left; trivial.
-                   right. unfold sharedTgt in H.
-                          rewrite sharedSrc_iff_frgnpub.
-                          apply orb_true_intro. 
-                          apply orb_prop in H.
-                          destruct H.
-                            left. intuition.
-                            right. intuition.
-               assumption.
-   split; assumption.
-Qed.*)
-(*eff_after_external - version using match_norm*)
-  clear core_diagram12 core_initial12 core_halted12 eff_diagram12 
-        core_diagram23 core_initial23 core_halted23 eff_diagram23
-        strong_diagram23 strong_diagram12 
-        strongperm_diagram23 strongperm_diagram12 (*match_eraseUnknown12 match_eraseUnknown23*).
+  eapply GLUEINV.
+(*after_external*)
+  clear - match_sm_wd12 match_sm_valid12 core_at_external12 eff_after_external12 
+          match_visible12 match_restrict12
+          match_sm_wd23 match_sm_valid23 core_at_external23 eff_after_external23.
   intros. rename st2 into st3. rename m2 into m3. 
           rename vals2 into vals3'. rename m2' into m3'.
           rename UnchLOOR into UnchLOOR13.
@@ -865,7 +485,7 @@ Qed.*)
   remember (fun b => locBlocksSrc mu12 b || frgnBlocksSrc mu12 b || mapped (as_inj (compose_sm mu12 mu23)) b)
       as RESTR.
   assert (NormMC12: match_core12 d12 (restrict_sm mu12 RESTR) st1 m1 st2 m2).
-     apply match_erase12. apply MC12.
+     apply match_restrict12. apply MC12.
      subst RESTR. clear. intuition.
      subst RESTR.
      clear UnchLOOR13 UnchPrivSrc Mu'Hyp mu' frgnTgtHyp frgnTgt'
@@ -873,9 +493,7 @@ Qed.*)
               SMvalNu' WDnu' SEP INC m3' ret2 m1' ret1 nu' NuHyp nu
               pubTgtHyp pubTgt' pubSrcHyp pubSrc' ValInjMu AtExtTgt 
               AtExtSrc eff_after_external23 core_at_external23 
-              match_genv23 genvs_dom_eq23 
-              eff_after_external12 core_at_external12
-              match_genv12 genvs_dom_eq12. 
+              eff_after_external12 core_at_external12. 
      subst. intros b Hb. rewrite REACHAX in Hb.
       destruct Hb as [L HL].
       generalize dependent b.
@@ -884,7 +502,7 @@ Qed.*)
       specialize (IHL _ H1); clear H1.
         apply orb_true_iff in IHL. apply orb_true_iff.
         destruct IHL.
-          left. eapply (match_norm12 _ _ _ _ _ _ MC12).
+          left. eapply (match_visible12 _ _ _ _ _ _ MC12).
                 eapply REACH_cons; try eassumption.
                 apply REACH_nil. apply H.
           right. eapply (inject_REACH_closed _ _ _ MemInjMu).
@@ -897,9 +515,7 @@ Qed.*)
               SMvalNu' WDnu' SEP INC m3' ret2 m1' ret1 nu' NuHyp nu
               pubTgtHyp pubTgt' pubSrcHyp pubSrc' ValInjMu AtExtTgt 
               AtExtSrc eff_after_external23 core_at_external23 
-              match_genv23 genvs_dom_eq23 
-              eff_after_external12 core_at_external12
-              match_genv12 genvs_dom_eq12. 
+              eff_after_external12 core_at_external12. 
       subst nmu12 mu RESTR. unfold compose_sm; simpl.
           rewrite restrict_sm_extern.
           rewrite (restrict_sm_local' _ WDmu12).
@@ -936,9 +552,9 @@ Qed.*)
     eapply compose_sm_wd; try eassumption.
       subst. unfold restrict_sm, restrict; simpl. destruct mu12; simpl in *. apply GLUEINV.
       subst. unfold restrict_sm, restrict; simpl. destruct mu12; simpl in *. apply GLUEINV.
-  clear match_norm12 match_norm12.
-  assert (mu12_valid:= match_validblock12 _ _ _ _ _ _ NormMC12).
-  assert (mu23_valid:= match_validblock23 _ _ _ _ _ _ MC23).
+  clear match_restrict12 match_visible12.
+  assert (mu12_valid:= match_sm_valid12 _ _ _ _ _ _ NormMC12).
+  assert (mu23_valid:= match_sm_valid23 _ _ _ _ _ _ MC23).
   rename ret2 into ret3.  
   destruct (core_at_external12 _ _ _ _ _ _ _ _ _ NormMC12 AtExtSrc)
    as [MInj12 [vals2 [ArgsInj12 (*[ArgsHT2*) AtExt2(*]*)]]]; clear core_at_external12.
@@ -985,7 +601,7 @@ Qed.*)
    remember (fun b => locBlocksSrc mu23 b && 
              REACH m2 (exportedSrc mu23 vals2) b) as pubSrcMid'.
    assert (MID: forall b, pubTgtMid' b = true -> pubSrcMid' b = true).
-        clear eff_after_external12 match_validblock23 eff_after_external23.
+        clear eff_after_external12 match_sm_valid23 eff_after_external23.
         rewrite HeqpubTgtMid', HeqpubSrcMid'. 
         destruct GLUEINV as [GlueA [GlueB [GlueC GlueD]]].
         subst.
@@ -1020,18 +636,43 @@ Qed.*)
      rewrite replace_locals_as_inj. assumption.
   assert (MinjNu23: Mem.inject (as_inj (replace_locals mu23 pubSrcMid' pubTgt')) m2 m3).
      rewrite replace_locals_as_inj. assumption.
+  assert (ArgsInj12R: Forall2
+    (val_inject
+       (as_inj
+          (restrict_sm mu12
+             (fun b : block =>
+              locBlocksSrc mu12 b || frgnBlocksSrc mu12 b
+              || mapped (as_inj (compose_sm mu12 mu23)) b)))) vals1 vals2).
+      clear - ArgsInj12 Heqnmu12 HeqRESTR.
+      rewrite restrict_sm_all. subst. rewrite restrict_sm_all in ArgsInj12.
+       rewrite restrict_nest in ArgsInj12.
+       eapply val_list_inject_forall_inject.
+       apply forall_inject_val_list_inject in ArgsInj12.
+       eapply val_list_inject_incr; try eassumption.
+       red; intros. destruct (restrictD_Some _ _ _ _ _ H); clear H.
+          unfold vis in H1. rewrite restrict_sm_locBlocksSrc, restrict_sm_frgnBlocksSrc in H1.
+          apply restrictI_Some; intuition.
+    intros. rewrite effect_properties.vis_restrict_sm in H.
+      unfold vis in H. intuition. 
+  clear ArgsInj12.
   assert (WDnu12: SM_wd (replace_locals nmu12 pubSrc' pubTgtMid')).
        subst.
        eapply replace_locals_wd; try eassumption.
          intros. apply andb_true_iff in H.
            destruct H as [locB R].
            destruct (REACH_local_REACH _ WDnmu12 _ _ _ _ 
-              MInj12 ArgsInj12 _ R locB) as [b2 [d1 [LOC12 R2]]].
+              MInj12 ArgsInj12R _ R locB) as [b2 [d1 [LOC12 R2]]].
            exists b2, d1; split; trivial.
            rewrite andb_true_iff, R2.
            split; trivial.
            eapply local_locBlocks; eassumption.
          intros. apply andb_true_iff in H. apply H. 
+  assert (ArgsInj23R: Forall2 (val_inject (as_inj mu23)) vals2 vals3).
+       eapply val_list_inject_forall_inject.
+       apply forall_inject_val_list_inject in ArgsInj23.
+       eapply val_list_inject_incr; try eassumption.
+       apply restrict_incr.
+  clear ArgsInj23.
   assert (WDnu23: SM_wd (replace_locals mu23 pubSrcMid' pubTgt')).
        subst. 
        eapply replace_locals_wd; try eassumption.
@@ -1039,7 +680,7 @@ Qed.*)
        intros b2; intros. apply andb_true_iff in H.
            destruct H as [locB R].
            destruct (REACH_local_REACH _ WDmu23 _ _ _ _ 
-              MInj23 ArgsInj23 _ R locB) as [b3 [d2 [LOC23 R3]]].
+              MInj23 ArgsInj23R _ R locB) as [b3 [d2 [LOC23 R3]]].
            exists b3, d2; split; trivial.
            rewrite andb_true_iff, R3.
            split; trivial.
@@ -1082,9 +723,7 @@ Qed.*)
               SMvalNu' WDnu' SEP INC m3' m1' ret1 nu' 
               pubTgtHyp pubSrcHyp ValInjMu AtExtTgt 
               AtExtSrc eff_after_external23 
-              match_genv23 genvs_dom_eq23 
-              eff_after_external12 MinjNu23
-              match_genv12 genvs_dom_eq12. 
+              eff_after_external12 MinjNu23. 
       destruct (extern_DomRng _ WDmu12 _ _ _ EX12).
       rewrite (extBlocksSrc_locBlocksSrc _ WDmu12 _ H) in RR; simpl in *.
       remember (frgnBlocksSrc mu12 b1) as d.
@@ -1195,4 +834,4 @@ Qed.*)
    split; assumption.
 Qed.
 
-End Eff_sim_trans.
+End Eff_sim_trans. 
